FunctorExamples/FunctorExample.i.dfy
@@ -1,0 +1,61 @@
+abstract module TIfc {
+  type TransitionLabel(==)
+}
+
+abstract module StateMachine(Ifc:TIfc) {
+  type Vars(==, !new)
+  predicate Init(s:Vars)
+  predicate Next(s:Vars, s':Vars, transition:Ifc.TransitionLabel)
+}
+
+module IncrementIfc refines TIfc {
+  datatype TransitionLabel = Inc(amt: int)
+}
+
+module IncrementSM refines StateMachine(IncrementIfc) {
+  datatype Vars = Vars(v: int)
+  import IncrementIfc
+  predicate Init(s:Vars) {
+    s.v == 0
+  }
+  predicate Next(s:Vars, s':Vars, transition:IncrementIfc.TransitionLabel) {
+    s'.v == s.v + transition.amt
+  }
+}
+
+abstract module StateMachinesRefine(L:StateMachine, H:StateMachine)
+  requires L.Ifc == H.Ifc  // XXX not yet supported
+{
+
+  // Implementation must supply an interpretation function.
+  function I(s:L.Vars) : H.Vars
+
+  // Implementation provides an invariant to support induction.
+  predicate Inv(s:L.Vars)
+
+  lemma InterpPreservesInit(s:L.Vars)
+      requires L.Init(s)
+      ensures H.Init(I(s))
+
+  lemma InvInit(s:L.Vars)
+      requires L.Init(s)
+      ensures Inv(s)
+
+  lemma InvNext(s:L.Vars, s':L.Vars, transition:L.Ifc.TransitionLabel)
+      requires Inv(s)
+      requires L.Next(s, s', transition)
+      ensures Inv(s')
+      ensures H.Next(I(s), I(s'), transition)
+}
+
+abstract module StateMachinesRefineTransitive(LR:StateMachinesRefine, HR:StateMachinesRefine)
+  refines StateMachinesRefine(LR.L, HR.H)
+  requires LR.H == HR.L  // XXX not yet supported
+{
+  // Implementation must supply an interpretation function.
+  function I(s:LR.L.Vars) : HR.H.Vars {
+    HR.I(LR.I(s))
+  }
+}
+
+
