FunctorExamples/FunctorRegret.i.dfy
@@ -1,0 +1,50 @@
+abstract module UIfc {
+  type UIOp(==)
+}
+
+abstract module UIStateMachine/*(Ifc:UIfc)*/ {
+  import Ifc : UIfc
+
+  type Vars(==, !new)
+  predicate Init(s:Vars)
+  predicate Next(s:Vars, s':Vars, uiop:Ifc.UIOp)
+}
+
+// The "unwinding condition" necessary to prove the TLA expression:
+// L.Init && []L.Next ==> H.Init && []H.Next
+abstract module StateMachinesRefine/*(Ifc: UIfc, L:UIStateMachine(Ifc), H:UIStateMachine(Ifc))*/ {
+  import Ifc : UIfc
+
+  // Error: module Ifc does not exist
+//  module UIStateMachineIfc refines UIStateMachine {
+//    import Ifc = Ifc
+//  }
+//  import L : UIStateMachineIfc
+//  import H : UIStateMachineIfc
+
+// Error: type mismatch for argument 2 (function expects Ifc.UIOp, got Ifc.UIOp)
+// There are now three unbound Ifcs floating around, not one.
+  import L : UIStateMachine
+  import H : UIStateMachine
+
+  // Implementation must supply an interpretation function.
+  function I(s:L.Vars) : H.Vars
+
+  // Implementation provides an invariant to support induction.
+  predicate Inv(s:L.Vars)
+
+  lemma InterpPreservesInit(s:L.Vars)
+      requires L.Init(s)
+      ensures H.Init(I(s))
+
+  lemma InvInit(s:L.Vars)
+      requires L.Init(s)
+      ensures Inv(s)
+
+  lemma InvNext(s:L.Vars, s':L.Vars, uiop:Ifc.UIOp)
+      requires Inv(s)
+      requires L.Next(s, s', uiop)
+      ensures Inv(s')
+      ensures H.Next(I(s), I(s'), uiop)
+}
+
