FunctorExamples/ModuleInstantiation.i.dfy
@@ -1,0 +1,29 @@
+abstract module TeamIfc {
+    type TeamMember(==)
+    type TeeShirtColor(==)
+}
+
+module TrainTeam refines TeamIfc {
+    datatype TeamMember = Engineer | Conductor | Brakeperson
+    function GetLeader() : TeamMember { Conductor }
+}
+
+abstract module UnionIfc refines TeamIfc {
+    function GetRepresentative(member: TeamMember) : TeamMember
+    {
+        var rep:TeamMember :| true; rep
+    }
+}
+
+module UnionizedTrain refines UnionIfc {
+    // This tells us what sauce satisfies SandwichIfc.TeamIfc.Sauce,
+    // which is why we can call TeamIfc.Pour.
+    // But SandwichIfc.Spread now expects CubanSauce, but
+    // TeamIfc.Pour is somehow a different type.
+    import TeamIfc = TrainTeam
+    // type TeamMember = TeamIfc.TeamMember // disallowed by Jon
+
+    function GetRepForLeader() : TeamMember {
+        GetRepresentative(TeamIfc.GetLeader())
+    }
+}
