FunctorExamples/ModuleSystemFrustration.i.dfy
@@ -1,0 +1,263 @@
+include "../lib/Base/Option.s.dfy"
+include "../lib/Base/sequences.i.dfy"
+
+/*
+ * What I want in a module system:
+ * The ability to refine multiple modules at once, specifying how imports from
+ * one satisfy abstract obligations (eg unstated types) of others.
+ *
+ * These definitions give rise to a family of related types, and I want to drop
+ * them in.
+ *
+ * Given that I'm stuck with Dafny's crappy one, I can rewrite this with templates,
+ * maybe. Nope, because templates don't provide a sane way to leave a parameter
+ * to be filled by a predicate body.
+ */
+
+abstract module UIfc {
+  type UIOp(==)
+}
+
+module MapIfc refines UIfc {
+  type K(==)
+  type V(==)
+  datatype UIOp = Put(k:K, v:V) | Get(k:K, v:V)
+}
+
+abstract module CrashableIfc refines UIfc {
+  type SyncId = nat
+  datatype CUIOp<UIOp> =
+    App(a:UIOp) | Crash | SyncRequest(syncId:SyncId) | SyncComplete(syncId:SyncId)
+}
+
+module CrashableMapIfc refines CrashableIfc {
+  
+}
+
+abstract module Spec {
+  import Ifc : UIfc
+
+  type Vars(==)
+  predicate Init(s:Vars)
+  predicate Next(s:Vars, s':Vars, uiop:Ifc.UIOp)
+}
+
+module MapSpec refines Spec {
+  import Ifc = MapIfc
+
+  type V = Ifc.V
+  type K = Ifc.K
+  // type UIOp = Ifc.UIOp // That I can't use this synonym is a bug.
+
+  datatype Vars = Vars(m:map<K,V>)
+  predicate Init(s:Vars) {
+    s.m == map[]
+  }
+  predicate Next(s:Vars, s':Vars, uiop:Ifc.UIOp) {
+    match uiop
+      case Get(k,v) => s.m[k]==v && s'==s
+      case Put(k,v) => s'.m == s.m[k := v]
+  }
+}
+
+// Analog to Spec
+abstract module Crashable refines CrashableIfc {
+  type Vars(==)
+  predicate Init(s:Vars)
+  predicate Next(s:Vars, s':Vars, iop:UIOp)
+}
+
+abstract module CrashSafe refines Crashable {
+  import opened Options
+  import opened Sequences
+
+  // The parameter machine
+  type PUIOp(==)
+  type PVars(==, !new)
+  predicate PInit(s:PVars)
+  predicate PNext(s:PVars, s':PVars, iop:PUIOp)
+
+  type AppOp = PUIOp
+
+  datatype View = View(p:PVars, syncId:Option<SyncId>)
+
+  // The sequence of states that have been issued toward the disk.
+  // The first one is persistent. The last one is the current ephemeral state.
+  // The ephemeral state always has syncId.None?.
+  datatype Vars = Vars(views:seq<View>)
+
+  predicate Init(s:Vars) {
+    && |s.views| == 1
+    && PInit(s.views[0].p)
+    && s.views[0].syncId.None?
+  }
+
+  predicate Next(s:Vars, s':Vars, uiop:UIOp) {
+    // spontaneous write completion can happen whenever you like
+    || s'.views == s.views[1..]
+    || (
+      && uiop.App?
+      && var e := Last(s.views).p;
+          exists e' ::
+            && PNext(e, e', uiop.a)
+            && s'.views == s.views + [View(e', None)]
+       )
+
+//    || (match uiop
+//        App(a) => (
+//          var e := Last(s.views).p;
+//          exists e' ::
+//            && PNext(e, e')
+//            && s'.views == s.views + [View(e', None)]
+//            )
+//
+//        Crash =>
+//          s'.views == s.views[..1]
+//          
+//        SyncRequest(syncId) =>
+//          var eview := Last(s.views);
+//          s'.views == DropLast(s.views) + [View(eview.p, syncId), eview]
+//
+//        SyncComplete(syncId) =>
+//          // If syncId is associated with the peristent state, you may report it complete.
+//          && s.views[0].syncId == syncId
+//          && s'.views == s.views[0 := s.views[0](.syncId == None)]
+//      )
+  }
+}
+
+module CrashSafeMap refines Crashable {
+  import opened MapSpec
+}
+
+//--module DiskIfc {
+//--  type Addr(!new, ==)
+//--  type Block(!new)
+//--  datatype IOp = Read(a:Addr, b:Block) | Write(a:Addr, b:Block)
+//--}
+//--
+//--module Disk {
+//--  import opened DiskIfc
+//-- 
+//--  datatype Vars = Vars(m:map<Addr, Block>)
+//--
+//--  predicate Next(s:Vars, s':Vars, iop:IOp) {
+//--    match iop
+//--      case Read(a, b) => a in s.m && s.m[a]==b && s'==s
+//--      case Write(a, b) => s'.m == s.m[a := b]
+//--  }
+//--}
+//--
+//--abstract module CacheIfc {
+//--  type Vars(!new)
+//--}
+//--
+//--abstract module ClientSkeleton {
+//--  import opened CrashableSpec
+//--  import opened DiskIfc
+//--  import Disk
+//--  import CacheIfc
+//--
+//--  type ConcreteVars
+//--  datatype Vars = Vars(cv:ConcreteVars, cache:CacheIfc.Vars)
+//--
+//--  predicate Init(s:Vars)
+//--  predicate Mkfs(d:Disk.Vars)
+//--  predicate Next(s:Vars, s':Vars, uiop:UIOp, iop:IOp)
+//--}
+//--
+//--abstract module CrashFreeIOSystem {
+//--  import opened CrashableSpec
+//--  import ClientSkeleton
+//--  import opened DiskIfc
+//--  import Disk
+//--
+//--  datatype Vars = Vars(c:ClientSkeleton.Vars, d:Disk.Vars)
+//--
+//--  predicate Init(s:Vars)
+//--  {
+//--    && ClientSkeleton.Init(s.c)
+//--    && ClientSkeleton.Mkfs(s.d)
+//--  }
+//--
+//--  predicate Next(s:Vars, s':Vars, uiop:UIOp, iop:IOp)
+//--  {
+//--    && !uiop.Crash?
+//--    && ClientSkeleton.Next(s.c, s'.c, uiop, iop)
+//--    && Disk.Next(s.d, s'.d, iop)
+//--  }
+//--}
+//--
+//--abstract module CrashableIOSystem {
+//--  import opened CrashableSpec
+//--  import ClientSkeleton
+//--  import opened DiskIfc
+//--  import Disk
+//--
+//--  datatype Vars = Vars(c:ClientSkeleton.Vars, d:Disk.Vars)
+//--
+//--  predicate Init(s:Vars)
+//--  {
+//--    && ClientSkeleton.Init(s.c)
+//--    && ClientSkeleton.Mkfs(s.d)
+//--  }
+//--
+//--  predicate Next(s:Vars, s':Vars, uiop:UIOp, iop:IOp)
+//--  {
+//--    if uiop.Crash?
+//--    then
+//--      && uiop.Crash?
+//--      && ClientSkeleton.Init(s'.c)
+//--      && s'.d == s'.d
+//--    else
+//--      && ClientSkeleton.Next(s.c, s'.c, uiop, iop)
+//--      && Disk.Next(s.d, s'.d, iop)
+//--  }
+//--}
+//--
+//--
+//--abstract module CrashSafeSpec refines CrashSafe {
+//-- 
+//--}
+//--
+//--abstract module CrashFreeIOSystemRefinement refines CrashFreeIOSystem {
+//--  import Spec
+//--
+//--  function I(s:Vars) : Spec.Vars
+//--}
+//--
+//--abstract module CrashableIOSystemRefinement refines CrashableIOSystem {
+//--  import Spec
+//--
+//--  function I(s:Vars) : Spec.Vars
+//--}
+//--
+//--abstract module CrashSafeCacheConfersCrashSafety {
+//--  import CrashFreeIOSystemRefinement
+//--  import CrashableIOSystemRefinement
+//--  import CrashableIOSystem
+//--  import CrashSafeSpec
+//--  import Spec
+//--
+//--  lemma CrashSafeCacheConfersCrashSafety()
+//--    requires
+//--      //var x : CrashFreeIOSystemRefinement.UIOp :| true;
+//--      var x := CrashFreeIOSystemRefinement.foo();
+//--      var y : Spec.UIOp :| true;
+//--      y==x
+//--    /*
+//--    requires forall s,s',uiop:CrashFreeIOSystemRefinement.UIOp,iop::
+//--      CrashFreeIOSystemRefinement.Next(s,s',uiop,iop)
+//--        ==> Spec.Next(CrashFreeIOSystemRefinement.I(s), CrashFreeIOSystemRefinement.I(s'), uiop)
+//--
+//--    // Try to bind Client the same way in both?
+//--    requires forall s,s',uiop,iop ::
+//--      CrashFreeIOSystemRefinement.ClientSkeleton.Next(s,s',uiop,iop)
+//--        <==> CrashableIOSystem.ClientSkeleton.Next(s,s',uiop,iop)
+//--
+//--    ensures forall s,s',uiop,iop ::
+//--      CrashableIOSystem.Next(s,s',uiop,iop)
+//--        ==> CrashSafeSpec.Next(CrashableIOSystemRefinement.I(s), CrashableIOSystemRefinement.I(s'), uiop)
+//--    */
+//--
+//--}
