FunctorExamples/RfcClean.i.dfy
@@ -1,0 +1,35 @@
+abstract module TIfc {
+  type TransitionLabel(==)
+}
+
+abstract module UIStateMachine(Ifc:TIfc) {
+  type Vars(==, !new)
+  predicate Init(s:Vars)
+  predicate Next(s:Vars, s':Vars, transition:Ifc.TransitionLabel)
+}
+
+abstract module StateMachinesRefine(
+    Ifc: TIfc,
+    L:UIStateMachine(Ifc),
+    H:UIStateMachine(Ifc)) {
+
+  // Implementation must supply an interpretation function.
+  function I(s:L.Vars) : H.Vars
+
+  // Implementation provides an invariant to support induction.
+  predicate Inv(s:L.Vars)
+
+  lemma InterpPreservesInit(s:L.Vars)
+      requires L.Init(s)
+      ensures H.Init(I(s))
+
+  lemma InvInit(s:L.Vars)
+      requires L.Init(s)
+      ensures Inv(s)
+
+  lemma InvNext(s:L.Vars, s':L.Vars, transition:Ifc.TransitionLabel)
+      requires Inv(s)
+      requires L.Next(s, s', transition)
+      ensures Inv(s')
+      ensures H.Next(I(s), I(s'), transition)
+}
