FunctorExamples/RfcWorkaround.i.dfy
@@ -1,0 +1,36 @@
+abstract module TIfc {
+  type TransitionLabel(==)
+}
+abstract module UIStateMachine {
+  import Ifc : TIfc
+  type Vars(==, !new)
+  predicate Init(s:Vars)
+  predicate Next(s:Vars, s':Vars, transition:Ifc.TransitionLabel)
+}
+
+abstract module UIParam refines TIfc {}
+
+abstract module LParam refines UIStateMachine {
+  import UIParam
+  import Ifc = UIParam
+}
+
+abstract module HParam refines UIStateMachine {
+  import UIParam
+  import Ifc = UIParam
+}
+
+abstract module StateMachinesRefine
+{
+  import L : LParam
+  import H : HParam
+
+  function I(s:L.Vars) : H.Vars
+  predicate Inv(s:L.Vars)
+  /* ... */
+  lemma InvNext(s:L.Vars, s':L.Vars, transition:L.Ifc.TransitionLabel)
+      requires Inv(s)
+      requires L.Next(s, s', transition)
+      ensures Inv(s')
+      ensures H.Next(I(s), I(s'), transition)
+}
