FunctorExamples/RobMarshallingExample.i.dfy
@@ -1,0 +1,24 @@
+abstract module Marshalling {
+  type Thing
+}
+
+abstract module IntegerMarshalling refines Marshalling {
+  type Thing = int
+}
+
+module Uint32Marshalling refines IntegerMarshalling {
+}
+
+abstract module SeqMarshalling(ElementMarshalling : Marshalling)
+{
+  type Booger
+}
+
+abstract module IntegerSeqMarshalling(IM : IntegerMarshalling) refines SeqMarshalling(IntegerMarshalling)
+{
+  type Doo = ElementMarshalling.Thing
+}
+
+//module Uint32SeqMarshalling refines IntegerSeqMarshalling(Uint32Marshalling)
+//{
+//}
