FunctorExamples/RobRefinesNotOpened.i.dfy
@@ -1,0 +1,15 @@
+abstract module A {
+  type X
+}
+
+abstract module B refines A {
+  predicate foo(x: X) {
+    true
+  }
+}
+
+abstract module C(D:A) {
+  predicate foo(x: D.X) {
+    true
+  }
+}
